books/projects/smtlink/verified/typed-term-mrg.lisp
@@ -1,0 +1,1701 @@
+;; Copyright (C) 2015, University of British Columbia
+;; Written by Yan Peng (December 30th 2019)
+;;
+;; License: A 3-clause BSD license.
+;; See the LICENSE file distributed with ACL2
+;;
+
+(in-package "SMT")
+(include-book "std/util/bstar" :dir :system)
+(include-book "xdoc/top" :dir :system)
+(include-book "std/util/define" :dir :system)
+(include-book "centaur/fty/top" :dir :system)
+(include-book "tools/defevaluator-fast" :dir :system)
+(include-book "clause-processors/just-expand" :dir :system)
+(include-book "clause-processors/meta-extract-user" :dir :system)
+(include-book "ordinals/lexicographic-ordering-without-arithmetic" :dir :system)
+
+(include-book "../utils/pseudo-term")
+(include-book "path-cond")
+(include-book "term-substitution")
+;; (include-book "evaluator")
+
+;; reduce not's in term
+(define simple-transformer ((term pseudo-termp))
+  :returns (new-term pseudo-termp)
+  (b* ((term (pseudo-term-fix term))
+       (new-term
+        (case-match term
+          (('not ('not term1)) term1)
+          (& term))))
+    new-term))
+
+(defsection |these-theorems-should-move-to-../utils/pseudo-term|
+  ;; mrg:  I needed these for some of the theorems that I added.
+  (defthm consp-of-pseudo-term-list-fix
+    (implies (consp x)
+             (consp (pseudo-term-list-fix x)))
+    :hints(("Goal" :expand (pseudo-term-list-fix x))))
+
+  (defthm null-of-pseudo-term-list-fix
+    (implies (not (consp x))
+             (equal (pseudo-term-list-fix x) nil))
+    :hints(("Goal" :expand (pseudo-term-list-fix x))))
+
+  (defthm len-of-pseudo-term-list-fix
+    (equal (len (pseudo-term-list-fix x))
+           (len x))
+    :hints(("Goal" :in-theory (enable pseudo-term-list-fix)))))
+
+(defsection |maybe-I-want-to-change-the-definition-of-is-conjunct?|
+  ;; I suspect that reasoning about is-conjunct? will be easier with
+  ;; the property below.  We could probably modify is-conjunct? to
+  ;; test (equal (cddddr term) nil) instead of (equal (len term) 4).
+  ;; That would be changing two lines of code instead of proving
+  ;; four theorems.
+  (local (defthm lemma-1
+           (implies (equal (len term) 4)
+                    (not (consp (cddddr term))))
+           :hints(("Goal"
+                   :in-theory (disable len)
+                   :expand ((len term)
+                            (len (cdr term))
+                            (len (cdr (cdr term)))
+                            (len (cdr (cdr (cdr term))))
+                            (len (cdr (cdr (cdr (cdr term))))))))))
+
+  (defthm cddddr-when-is-conjunct?
+    (implies (is-conjunct? term)
+             (not (consp (cddddr term))))
+    :hints(
+           ("Goal"
+            :in-theory (disable len pseudo-termp lemma-1)
+            :use((:instance lemma-1))
+            :expand(
+                    (is-conjunct? term)
+                    (pseudo-term-fix term))))))
+
+(defsection typed-term
+  (local (in-theory (disable pseudo-termp)))
+
+  (defprod typed-term
+    ((term pseudo-termp :default ''nil)
+     (path-cond pseudo-termp :default ''t)
+     (judgements pseudo-termp :default '(if (if (symbolp 'nil)
+                                                (if (booleanp 'nil) 't 'nil)
+                                              'nil)
+                                            't
+                                          'nil))))
+
+  (deflist typed-term-list
+    :elt-type typed-term-p
+    :true-listp t)
+
+  (define typed-term-list->term-lst ((tterm-lst typed-term-list-p))
+    :measure (len (typed-term-list-fix tterm-lst))
+    :returns (term-lst pseudo-term-listp)
+    (b* ((tterm-lst (typed-term-list-fix tterm-lst))
+         ((unless (consp tterm-lst)) nil)
+         ((cons tterm-hd tterm-tl) tterm-lst)
+         ((typed-term tth) tterm-hd))
+      (cons tth.term (typed-term-list->term-lst tterm-tl)))
+    ///
+    (more-returns
+     (term-lst
+      (equal (acl2-count
+              (typed-term-list->term-lst (typed-term-list-fix tterm-lst)))
+             (acl2-count term-lst))
+      :name acl2-count-equal-of-typed-term-list-fix
+      :hints (("Goal"
+               :expand (typed-term-list->term-lst tterm-lst))))
+     (term-lst
+      (implies (consp tterm-lst)
+               (< (acl2-count (typed-term->term (car tterm-lst)))
+                  (acl2-count term-lst)))
+      :name acl2-count-of-car-of-typed-term-list-p)
+     (term-lst
+      (implies (typed-term-list-p tterm-lst)
+               (equal (len term-lst) (len tterm-lst)))
+      :name typed-term-list->term-lst-maintains-len)
+     ;; added by mrg
+     (term-lst (implies (consp tterm-lst) (consp term-lst))
+               :name consp-of-typed-term-lst->term-lst
+               :hints(("Goal" :in-theory (enable typed-term-list->term-lst))))
+     (term-lst (implies (not (consp tterm-lst)) (equal term-lst nil))
+               :name null-of-typed-term-lst->term-lst
+               :hints(("Goal" :in-theory (enable typed-term-list->term-lst))))))
+
+  (defthm acl2-count-of-cdr-of-typed-term-list-p
+    (implies (consp tterm-lst)
+             (< (acl2-count (typed-term-list->term-lst (cdr tterm-lst)))
+                (acl2-count (typed-term-list->term-lst tterm-lst))))
+    :hints (("Goal"
+             :expand (typed-term-list->term-lst tterm-lst))))
+
+  (define typed-term-list->judgements ((tterm-lst typed-term-list-p))
+    :measure (len (typed-term-list-fix tterm-lst))
+    :returns (judges pseudo-termp)
+    (b* ((tterm-lst (typed-term-list-fix tterm-lst))
+         ((unless (consp tterm-lst)) ''t)
+         ((cons tterm-hd tterm-tl) tterm-lst)
+         ((typed-term tth) tterm-hd))
+      `(if ,tth.judgements
+           ,(typed-term-list->judgements tterm-tl)
+         'nil)))
+
+  ;; mrg:  I removed the check for uniform-path-cond? because it
+  ;;   was forcing messy induction proofs when reasoning about
+  ;;   make-typed-term-list.  I suspect that this simpler version
+  ;;   typed-term-list->path-cond "works" for everything we need
+  ;;   anyway.
+  ;;     Then, I moved the definition of typed-term-list->path-cond
+  ;;   *before* uniform-path-cond? so I could use it in the definition
+  ;;   of uniform-path-cond?.  This makes subsequent proofs work
+  ;;   with fewer hints.
+  (define typed-term-list->path-cond ((tterm-lst typed-term-list-p))
+    :returns (path-cond pseudo-termp)
+    (b* ((tterm-lst (typed-term-list-fix tterm-lst))
+         ((unless (consp tterm-lst)) ''t)
+         ((cons tterm-hd &) tterm-lst)
+         ((typed-term tth) tterm-hd))
+      tth.path-cond))
+
+  ;; mrg:  added uniform-path-help because it makes reasoning about
+  ;;   uniform-path-cond? easier.  That's because uniform-path-help
+  ;;   has a "better" induction schema (by keeping path-cond unchanged).
+  (define uniform-path-help ((tterm-lst typed-term-list-p) (path-cond pseudo-termp))
+    :returns (ok booleanp)
+    (b* (((unless (consp tterm-lst)) t)
+         ((unless (equal (typed-term-list->path-cond tterm-lst) path-cond)) nil))
+      (uniform-path-help (cdr tterm-lst) path-cond))
+    ///
+    (more-returns
+     (ok (implies (not (consp tterm-lst)) ok)
+         :name uniform-path-help-of-atom)
+     (ok (implies ok (uniform-path-help (cdr tterm-lst) path-cond))
+         :name uniform-path-help-of-cdr
+         :hints(("Goal" :in-theory (enable uniform-path-help))))
+     (ok (implies (and ok (consp (cdr tterm-lst)))
+                  (and (equal (typed-term-list->path-cond (cdr tterm-lst)) path-cond)
+                       (equal (typed-term-list->path-cond tterm-lst) path-cond)))
+         :name uniform-path-help-when-len-geq-2
+         :hints(("Goal" :in-theory (enable uniform-path-help))))))
+
+  (define uniform-path-cond? ((tterm-lst typed-term-list-p))
+    :returns (ok booleanp)
+    (uniform-path-help tterm-lst (typed-term-list->path-cond tterm-lst))
+    ///
+    (more-returns
+     (ok (implies ok (uniform-path-cond? (cdr tterm-lst)))
+         :name uniform-path-cond?-of-cdr
+         :hints(("Goal" :cases(
+                               (and (consp tterm-lst) (consp (cdr tterm-lst)))
+                               (and (consp tterm-lst) (not (consp (cdr tterm-lst))))))))
+     (ok (implies (and (typed-term-list-p tterm-lst)
+                       (consp tterm-lst) (consp (cdr tterm-lst))
+                       ok)
+                  (equal (typed-term-list->path-cond (cdr tterm-lst))
+                         (typed-term-list->path-cond tterm-lst)))
+         :name equal-of-uniform-path-cond?)))
+
+
+  ;; make-typed-term-list-guard -- state the relationship that
+  ;; make-typed-term-list needs between term-lst and judges.
+  ;; By moving this into the guard, the body of make-typed-term-list
+  ;; doesn't need a bunch of ((if bad) (er ?hard ...)) bindings in its b*.
+  ;; That makes reasoning about make-typed-term-list easier.
+  (define make-typed-term-list-guard ((term-lst pseudo-term-listp)
+                                      (path-cond pseudo-termp)
+                                      (judges pseudo-termp))
+    :returns (ok booleanp)
+    :enabled t
+    (b* (((unless (pseudo-term-listp term-lst)) nil)
+         ((unless (pseudo-termp path-cond)) nil)
+         ((unless (pseudo-termp judges)) nil)
+         ((unless (is-conjunct? judges)) nil)
+         ((if (and (null term-lst) (equal judges ''t))) t)
+         ((if (or  (null term-lst) (equal judges ''t))) nil)
+         (term-tl (cdr term-lst))
+         ((list & & judge-tl &) judges)) ;; (if judge-hd judge-tl nil)
+      (make-typed-term-list-guard term-tl path-cond judge-tl))
+    ///
+    (more-returns
+     (ok (implies (and ok (consp term-lst))
+                  (make-typed-term-list-guard (cdr term-lst) path-cond (caddr judges)))
+         :name make-typed-term-list-guard-of-cdr
+         :hints(("Goal" :in-theory (enable make-typed-term-list-guard))))))
+
+  ;; make-typed-term-list-fix-judges
+  ;;   A "fixing" function to make judges satisfy make-typed-term-list-guard.
+  ;;   Takes about 20 seconds to define this function (2.6GHz, i5 Macbook Pro).
+  ;;   The main culprit is the more-returns theorem
+  ;;     make-typed-term-list-guard-of-make-typed-term-list-fix-judges
+  (define make-typed-term-list-fix-judges ((term-lst pseudo-term-listp)
+                                           (path-cond pseudo-termp)
+                                           (judges pseudo-termp))
+    :guard (make-typed-term-list-guard term-lst path-cond judges)
+    :returns (j-fix pseudo-termp)
+    :verify-guards nil
+    (mbe
+     :logic
+     (b* ((term-lst (pseudo-term-list-fix term-lst))
+          (path-cond (pseudo-term-fix path-cond))
+          (judges (pseudo-term-fix judges))
+          ((if (null term-lst)) ''t)
+          ((mv judge-hd judge-tl)
+           (if (and (is-conjunct? judges) (not (equal judges ''t)))
+               (mv (cadr judges) (caddr judges))
+             (mv ''t ''t)))
+          (jtl-fix (make-typed-term-list-fix-judges (cdr term-lst)
+                                                    path-cond
+                                                    judge-tl)))
+       `(if ,judge-hd ,jtl-fix 'nil))
+     :exec judges)
+    ///
+    ;; mrg:  the proof of idempotence-of-make-typed-term-list-fix-judges
+    ;;   fails when stated as a more-returns theorem but succeeds ;   this way
+    (defthm idempotence-of-make-typed-term-list-fix-judges
+      (let ((j-fix (make-typed-term-list-fix-judges tterm-lst path-cond judges)))
+        (equal (make-typed-term-list-fix-judges tterm-lst path-cond j-fix) j-fix))
+      :hints(("Goal"
+              :in-theory (e/d (make-typed-term-list-fix-judges) (pseudo-termp)))))
+    (more-returns
+     (j-fix (make-typed-term-list-guard (pseudo-term-list-fix term-lst)
+                                        (pseudo-term-fix path-cond)
+                                        j-fix)
+            :name
+            make-typed-term-list-guard-of-make-typed-term-list-fix-judges)
+     ;; make-typed-term-list-judges-fix-when-make-typed-term-list-guard
+     ;; takes about 15 seconds to prove -- even if I give it a shorter name.
+     ;; That's kind of annoying.  Might want to figure out why (i.e. why it
+     ;; takes so long.  I know why waiting for the proof to finish is
+     ;; annoying)
+     ;; Yan: I disabled some rules, not it runs slightly faster
+     (j-fix (implies (make-typed-term-list-guard term-lst path-cond judges)
+                     (equal j-fix judges))
+            :name make-typed-term-list-judges-fix-when-make-typed-term-list-guard
+            :hints(("Goal" :in-theory (e/d (is-conjunct?
+                                            make-typed-term-list-fix-judges)
+                                           (symbol-listp
+                                            acl2::symbolp-of-car-when-symbol-listp
+                                            acl2::symbol-listp-of-cdr-when-symbol-listp))))))
+    (verify-guards make-typed-term-list-fix-judges
+      :hints(("Goal"
+              :in-theory (disable make-typed-term-list-judges-fix-when-make-typed-term-list-guard)
+              :use((:instance
+                    make-typed-term-list-judges-fix-when-make-typed-term-list-guard)))))
+    )
+
+
+  (define make-typed-term-list ((term-lst pseudo-term-listp)
+                                (path-cond pseudo-termp)
+                                (judges pseudo-termp))
+    :guard (make-typed-term-list-guard term-lst path-cond judges)
+    :returns (tterm-lst typed-term-list-p)
+    :guard-hints(("Goal"
+                  :expand ((make-typed-term-list-guard term-lst path-cond judges))))
+
+    (b* ((term-lst (pseudo-term-list-fix term-lst))
+         (path-cond (pseudo-term-fix path-cond))
+         (judges (make-typed-term-list-fix-judges term-lst path-cond judges))
+         ((unless (consp term-lst)) nil)
+         ((cons term-hd term-tl) term-lst)
+         ((list & judge-hd judge-tl &) judges))
+      (cons (make-typed-term :term term-hd :path-cond path-cond
+                             :judgements judge-hd)
+            (make-typed-term-list term-tl path-cond judge-tl)))
+    ///
+    ;; mrg: first, two lemmas about make-typed-term-list-fix-judges that
+    ;;   are needed for the proof of
+    ;;   typed-term-list->judgements-of-make-typed-term-list
+    (local (defthm lemma-j1
+             (implies (or (not (consp term-lst)) (not (consp (pseudo-term-list-fix term-lst))))
+                      (equal (make-typed-term-list-fix-judges term-lst path-cond judges)
+                             ''t))
+             :hints(("Goal" :expand((make-typed-term-list-fix-judges term-lst path-cond judges))))))
+
+
+    ;; mrg: lemma-j2 is a "cut-and-paste" lemma from a failed subgoal for
+    ;;   typed-term-list->judgements-of-make-typed-term-list.  The proof
+    ;;   feels a bit brittle.  See the comments in the theorem statement.
+    (local (defthm lemma-j2
+             (implies
+              ;; the writer doesn't find lemma-j2 if the hypothesis is (consp term-lst)
+              (consp (pseudo-term-list-fix term-lst))
+              ;; The proof of typed-term-list->judgements-of-make-typed-term-list fails
+              ;; with a rewrite loop if I don't use this (equal ... t) construction.
+              (equal
+               (equal (make-typed-term-list-fix-judges term-lst path-cond judges)
+                      (LIST
+                       'IF
+                       (PSEUDO-TERM-FIX
+                        (CADR (MAKE-TYPED-TERM-LIST-FIX-JUDGES (PSEUDO-TERM-LIST-FIX TERM-LST)
+                                                               (PSEUDO-TERM-FIX PATH-COND)
+                                                               JUDGES)))
+                       (MAKE-TYPED-TERM-LIST-FIX-JUDGES
+                        (CDR (PSEUDO-TERM-LIST-FIX TERM-LST))
+                        (PSEUDO-TERM-FIX PATH-COND)
+                        (CADDR (MAKE-TYPED-TERM-LIST-FIX-JUDGES (PSEUDO-TERM-LIST-FIX TERM-LST)
+                                                                (PSEUDO-TERM-FIX PATH-COND)
+                                                                JUDGES)))
+                       ''nil))
+               t))
+             :hints(("Goal"
+                     :expand(
+                             (make-typed-term-list-fix-judges term-lst path-cond judges)
+                             (MAKE-TYPED-TERM-LIST-FIX-JUDGES (PSEUDO-TERM-LIST-FIX TERM-LST)
+                                                              (PSEUDO-TERM-FIX PATH-COND)
+                                                              JUDGES))))))
+
+    (more-returns
+     ;; mrg: I changed acl2-count-of-typed-term-list->term-lst into a
+     ;;   more-returns theorem (it had been a defthm) for consistency
+     ;;   Note: we could also prove
+     ;;     (equal (len (make-typed-term-list term-lst path-cond judges))
+     ;;            (len term-lst))
+     ;;   If that would be useful in subsequent measure proofs.
+     (tterm-lst (<= (acl2-count (typed-term-list->term-lst tterm-lst))
+                    (acl2-count term-lst))
+                :name acl2-count-of-typed-term-list->term-lst
+                :hints(("Goal" :in-theory (enable typed-term-list->term-lst)))
+                :rule-classes :linear)
+     ;; mrg: I added the more-returns theorems from here to the end of
+     ;;      define make-typed-term-list.
+     (tterm-lst (implies (consp term-lst) (consp tterm-lst))
+                :name consp-of-make-typed-term-list
+                :hints(("Goal"
+                        :expand((make-typed-term-list term-lst path-cond judges)))))
+
+     (tterm-lst (implies (not (consp term-lst)) (equal tterm-lst nil))
+                :name null-of-make-typed-term-list
+                :hints(("Goal"
+                        :expand((make-typed-term-list term-lst path-cond judges)))))
+
+     (tterm-lst (implies (pseudo-term-listp term-lst)
+                         (equal (typed-term-list->term-lst tterm-lst) term-lst))
+                :name typed-term-list->term-lst-of-make-typed-term-list
+                :hints(("Goal" :in-theory (enable typed-term-list->term-lst))))
+
+     (tterm-lst (equal (typed-term-list->path-cond tterm-lst)
+                       (if (consp term-lst) (pseudo-term-fix path-cond) ''t))
+                :name typed-term-list->path-cond-of-make-typed-term-list
+                :hints(("Goal"
+                        :in-theory (enable typed-term-list->path-cond))))
+
+     (tterm-lst (equal (typed-term-list->judgements tterm-lst)
+                       (make-typed-term-list-fix-judges term-lst path-cond judges))
+                :name typed-term-list->judgements-of-make-typed-term-list
+                :hints(("Goal" :in-theory (enable typed-term-list->judgements))))
+
+     (tterm-lst (implies (pseudo-termp path-cond)
+                         (uniform-path-help tterm-lst path-cond))
+                :name uniform-path-help-of-make-typed-term-list
+                :hints(("Goal"
+                        :in-theory (enable uniform-path-help
+                                           make-typed-term-list
+                                           typed-term-list->path-cond))))
+
+     (tterm-lst (implies (pseudo-termp path-cond)
+                         (uniform-path-cond? tterm-lst))
+                :name uniform-path-cond?-of-make-typed-term-list
+                :hints(("Goal" :in-theory (enable uniform-path-cond?)))))))
+
+
+(defsection make-typed-term-list-from-fields
+  ;; mrg: my goal is to show that if tterm-lst is a typed-term-list-p
+  ;;   and tterm-list satisfies uniform-path-cond?, then 
+  ;;     (equal
+  ;;       (make-typed-term-list
+  ;;         (typed-term-list->term-lst tterm-lst)
+  ;;         (typed-term-list->path-cond tterm-lst)
+  ;;         (typed-term-list->judgements tterm-lst))
+  ;;     tterm-lst)
+  ;;   This is theorem make-typed-term-list-from-fields.
+  ;;   
+  ;;   Along the way, I prove a few other theorems that may be useful
+  ;;   outside of this defsection:
+  ;;     make-typed-term-list-guard-from-fields
+  ;;       this theorem states that make-typed-term-list-guard is
+  ;;       satisfied by
+  ;;         (typed-term-list->term-lst tterm-lst)
+  ;;         (typed-term-list->path-cond tterm-lst)
+  ;;         (typed-term-list->judgements tterm-lst)
+  ;;       no matter what tterm-lst is.  Aha, that's why I made the
+  ;;       the changes that I did to those functions for the cases
+  ;;       where tterm-lst is "bad".
+  ;;
+  ;;     car-of-make-typed-term-list
+  ;;       If tterm-list is a non-nil typed-term-list-p, then
+  ;;         (equal
+  ;;           (car (make-typed-term-list
+  ;;                 (typed-term-list->term-lst tterm-lst)
+  ;;                 (typed-term-list->path-cond tterm-lst)
+  ;;                 (typed-term-list->judgements tterm-lst)))
+  ;;           (car tterm-lst))
+  ;;       I don't need the uniform-path-cond? hypthesis here.
+
+  (local (in-theory (disable pseudo-termp)))
+  
+  (local (defthm lemma-1
+           (implies (pseudo-termp path-cond)
+                    (make-typed-term-list-guard
+                     (typed-term-list->term-lst tterm-lst)
+                     path-cond
+                     (typed-term-list->judgements tterm-lst)))
+           :hints(("Goal"
+                   :in-theory (enable
+                               make-typed-term-list-guard
+                               typed-term-list->term-lst
+                               typed-term-list->judgements)))))
+
+  (defthm make-typed-term-list-guard-from-fields
+    (make-typed-term-list-guard
+     (typed-term-list->term-lst tterm-lst)
+     (typed-term-list->path-cond tterm-lst)
+     (typed-term-list->judgements tterm-lst)))
+
+  ;; I don't want to enable typed-term-list->judgements for the
+  ;; proof of car-of-make-typed-term-list because it makes the
+  ;; terms for the :expand hint much messier.
+  (local (defthm lemma-2
+           (implies
+            (and (typed-term-list-p tterm-lst) (consp tterm-lst))
+            (and (equal (cadr (typed-term-list->judgements tterm-lst))
+                        (typed-term->judgements (car tterm-lst)))
+                 (equal (caddr (typed-term-list->judgements tterm-lst))
+                        (typed-term-list->judgements (cdr tterm-lst)))))
+           :hints(("Goal" :in-theory (enable typed-term-list->judgements)))))
+
+  (defthm car-of-make-typed-term-list
+    (let ((tterm-lst2 (make-typed-term-list (typed-term-list->term-lst tterm-lst)
+                                            (typed-term-list->path-cond tterm-lst)
+                                            (typed-term-list->judgements tterm-lst))))
+      (implies (and (typed-term-list-p tterm-lst) (consp tterm-lst))
+               (equal (car tterm-lst2)(car tterm-lst))))
+    :hints(("Goal"
+            :in-theory (disable make-typed-term-list-guard-from-fields)
+            :use((:instance make-typed-term-list-guard-from-fields))
+            :expand(
+                    (typed-term-list->term-lst tterm-lst)
+                    (typed-term-list->path-cond tterm-lst)
+                    (make-typed-term-list
+                     (cons (typed-term->term (car tterm-lst))
+                           (typed-term-list->term-lst (cdr tterm-lst)))
+                     (typed-term->path-cond (car tterm-lst))
+                     (typed-term-list->judgements tterm-lst))))))
+
+  (local (defthmd lemma-3
+           (implies (and (typed-term-list-p tterm-lst)
+                         (uniform-path-help tterm-lst path-cond)
+                         (pseudo-termp path-cond))
+                    (let* ((term-lst1  (typed-term-list->term-lst tterm-lst))
+                           (judges1    (typed-term-list->judgements tterm-lst))
+                           (tterm-lst1 (make-typed-term-list term-lst1 path-cond judges1))
+                           (term-lst2  (typed-term-list->term-lst (cdr tterm-lst)))
+                           (judges2    (typed-term-list->judgements (cdr tterm-lst)))
+                           (tterm-lst2 (make-typed-term-list term-lst2 path-cond judges2)))
+                      (equal tterm-lst2 (cdr tterm-lst1))))
+           :hints(("Goal"
+                   :in-theory (disable lemma-1)
+                   :use((:instance lemma-1))
+                   :expand(
+                           (typed-term-list->term-lst tterm-lst)
+                           (typed-term-list->path-cond tterm-lst)
+                           (typed-term-list->judgements tterm-lst)
+                           (make-typed-term-list
+                            (cons (typed-term->term (car tterm-lst))
+                                  (typed-term-list->term-lst (cdr tterm-lst)))
+                            path-cond
+                            (list* 'if
+                                   (typed-term->judgements (car tterm-lst))
+                                   (typed-term-list->judgements (cdr tterm-lst))
+                                   '('nil))))))))
+
+  (local (defthm crock-pain-0
+           (implies
+            (UNIFORM-PATH-HELP TTERM-LST (TYPED-TERM-LIST->PATH-COND TTERM-LST))
+            (equal (MAKE-TYPED-TERM-LIST (TYPED-TERM-LIST->TERM-LST (CDR TTERM-LST))
+                                         (TYPED-TERM-LIST->PATH-COND TTERM-LST)
+                                         (TYPED-TERM-LIST->JUDGEMENTS (CDR TTERM-LST)))
+                   (MAKE-TYPED-TERM-LIST (TYPED-TERM-LIST->TERM-LST (CDR TTERM-LST))
+                                         (TYPED-TERM-LIST->PATH-COND (cdr TTERM-LST))
+                                         (TYPED-TERM-LIST->JUDGEMENTS (CDR TTERM-LST)))))
+           :hints(("Goal"
+                   :cases((and (consp tterm-lst) (consp (cdr tterm-lst)))
+                          (and (consp tterm-lst) (not (consp (cdr tterm-lst)))))))))
+
+  (local (defthm crock-pain-1
+           (let ((tterm-lst2 (MAKE-TYPED-TERM-LIST (TYPED-TERM-LIST->TERM-LST TTERM-LST)
+                                                   (TYPED-TERM-LIST->PATH-COND TTERM-LST)
+                                                   (TYPED-TERM-LIST->JUDGEMENTS TTERM-LST))))
+             (IMPLIES
+              (and (EQUAL (MAKE-TYPED-TERM-LIST (TYPED-TERM-LIST->TERM-LST (CDR TTERM-LST))
+                                                (TYPED-TERM-LIST->PATH-COND (cdr TTERM-LST))
+                                                (TYPED-TERM-LIST->JUDGEMENTS (CDR TTERM-LST)))
+                          (CDR TTERM-LST))
+                   (TYPED-TERM-LIST-P TTERM-LST)
+                   (UNIFORM-PATH-HELP TTERM-LST (TYPED-TERM-LIST->PATH-COND TTERM-LST)))
+              (EQUAL (cdr tterm-lst2) (cdr TTERM-LST))))
+           :hints(
+                  ("Goal"
+                   :in-theory (disable lemma-3)
+                   :use(
+                        (:instance lemma-3 (path-cond (typed-term-list->path-cond tterm-lst))))))))
+
+  (local (defthmd crock-pain-2
+           (let ((tterm-lst2 (MAKE-TYPED-TERM-LIST (TYPED-TERM-LIST->TERM-LST TTERM-LST)
+                                                   (TYPED-TERM-LIST->PATH-COND TTERM-LST)
+                                                   (TYPED-TERM-LIST->JUDGEMENTS TTERM-LST))))
+             (implies
+              (and (typed-term-list-p tterm-lst) (consp tterm-lst) (consp tterm-lst2)
+                   (EQUAL (car tterm-lst2) (car tterm-lst))
+                   (EQUAL (cdr tterm-lst2) (cdr tterm-lst)))
+              (EQUAL tterm-lst2 tterm-lst)))
+           :hints(("Goal"
+                   :in-theory (disable car-of-make-typed-term-list consp-of-make-typed-term-list)))))
+
+  (local (defthm crock-pain-3
+           (let ((tterm-lst2 (MAKE-TYPED-TERM-LIST (TYPED-TERM-LIST->TERM-LST TTERM-LST)
+                                                   (TYPED-TERM-LIST->PATH-COND TTERM-LST)
+                                                   (TYPED-TERM-LIST->JUDGEMENTS TTERM-LST))))
+             (implies
+              (and (typed-term-list-p tterm-lst)
+                   (EQUAL (cdr tterm-lst2) (cdr tterm-lst)))
+              (equal tterm-lst2 tterm-lst)))
+           :hints(("Goal" :use((:instance crock-pain-2))))))
+
+  (local (defthm crock-pain-4
+           (let ((tterm-lst2 (MAKE-TYPED-TERM-LIST (TYPED-TERM-LIST->TERM-LST TTERM-LST)
+                                                   (TYPED-TERM-LIST->PATH-COND TTERM-LST)
+                                                   (TYPED-TERM-LIST->JUDGEMENTS TTERM-LST))))
+             (implies
+              (and (EQUAL (MAKE-TYPED-TERM-LIST (TYPED-TERM-LIST->TERM-LST (CDR TTERM-LST))
+                                                (TYPED-TERM-LIST->PATH-COND (cdr TTERM-LST))
+                                                (TYPED-TERM-LIST->JUDGEMENTS (CDR TTERM-LST)))
+                          (CDR TTERM-LST))
+                   (TYPED-TERM-LIST-P TTERM-LST)
+                   (UNIFORM-PATH-HELP TTERM-LST (TYPED-TERM-LIST->PATH-COND TTERM-LST)))
+              (equal tterm-lst2 tterm-lst)))))
+
+  (defthm make-typed-term-list-from-fields
+    (implies (and (typed-term-list-p tterm-lst)
+                  (uniform-path-cond?  tterm-lst))
+             (let* ((term-lst (typed-term-list->term-lst tterm-lst))
+                    (path-cond (typed-term-list->path-cond tterm-lst))
+                    (judges   (typed-term-list->judgements tterm-lst))
+                    (tterm-lst2 (make-typed-term-list term-lst path-cond judges)))
+               (equal tterm-lst2 tterm-lst)))
+    :hints(("Goal"
+            :in-theory (e/d (make-typed-term-list uniform-path-cond? uniform-path-help)
+                            (crock-pain-0 crock-pain-1 crock-pain-2 crock-pain-3))))))
+
+(defsection make-typed-term-list-fix-judges-when-term-lst-equal-len
+  ;; Another bunch of theorems to prove something that I intend to use later
+  ;; in this file.
+  ;;   (make-typed-term-list-fix-judges term-lst path-cond judges)
+  ;; is mostly concerned about judges.  There needs to be a correspondence
+  ;; between the conjuncts in judges and the terms in term-lst, but this
+  ;; means that the only thing that matters about term-lst is its length.
+  ;; Thus, we prove the congruence:
+  ;;   (implies (equal (len term-lst) (len term-lst-equiv))
+  ;;            (equal (make-typed-term-list-fix-judges term-lst path-cond judges)
+  ;;                   (make-typed-term-list-fix-judges term-lst-equiv path-cond judges)))
+  ;; We also introduce:
+  ;;   equal-len: an equivalence relation we need to state the main congruence.
+  ;;   equal-len-implies-equal-len-cdr-1:  a congruence, i.e. cdr preserves equal-len
+  ;;   equal-len-implies-equal-len-pseudo-term-list-fix-1:
+  ;;     same as len-of-pseudo-term-list-fix but stated as a congruence
+  ;;   equal-len-implies-iff-pseudo-term-list-fix-1:
+  ;;     same as null-of-pseudo-term-list-fix but stated as a congruence
+
+  (local (in-theory (disable pseudo-termp)))
+
+  (define equal-len (x y)
+    :enabled t
+    (equal (len x) (len y))
+    ///
+    (defequiv equal-len))
+
+  (defthm equal-len-of-pseudo-term-list-fix
+    (equal-len (pseudo-term-list-fix term-lst) term-lst))
+
+  (defcong equal-len iff (pseudo-term-list-fix term-lst) 1
+    :hints(("Goal"
+            :expand ((pseudo-term-list-fix term-lst)
+                     (pseudo-term-list-fix term-lst-equiv)))))
+
+  (defcong equal-len equal-len (cdr x) 1)
+  
+  (in-theory (disable equal-len))
+  (defcong equal-len equal
+    (make-typed-term-list-fix-judges term-lst path-cond judges) 1
+    :hints(("Goal" :in-theory (enable make-typed-term-list-fix-judges)))))
+
+;; ---------------------------------------------
+;;       Recognizers
+
+(local
+ (defthm type-of-0-input-fn
+   (implies (and (symbolp fn)
+                 (not (equal fn 'quote)))
+            (and (not (pseudo-lambdap `(,fn)))
+                 (pseudo-termp `(,fn))))
+   :hints (("Goal"
+            :in-theory (enable pseudo-lambdap)))))
+
+(define typed-term->kind ((tterm typed-term-p))
+  :returns (kind symbolp)
+  (b* ((tterm (typed-term-fix tterm))
+       ((typed-term tt) tterm)
+       ((if (acl2::variablep tt.term)) 'variablep)
+       ((if (acl2::quotep tt.term)) 'quotep)
+       ((cons fn &) tt.term)
+       ((if (pseudo-lambdap fn)) 'lambdap)
+       ((if (equal fn 'if)) 'ifp))
+    'fncallp)
+  ///
+  (more-returns
+   (kind (member-equal kind '(variablep quotep lambdap ifp fncallp))
+         :name range-of-typed-term->kind)
+   (kind (implies (and (typed-term-p tterm)
+                       (not (equal kind 'variablep))
+                       (not (equal kind 'quotep))
+                       (not (equal kind 'lambdap))
+                       (not (equal kind 'ifp)))
+                  (equal kind 'fncallp))
+         :name cases-of-typed-term->kind)
+   (kind (implies (equal kind 'variablep)
+                  (acl2::variablep (typed-term->term tterm)))
+         :name implies-of-variable-kind)
+   (kind (implies (equal kind 'quotep)
+                  (acl2::quotep (typed-term->term tterm)))
+         :name implies-of-quote-kind)
+   (kind (implies (equal kind 'lambdap)
+                  (and (consp (typed-term->term tterm))
+                       (pseudo-lambdap (car (typed-term->term tterm)))))
+         :name implies-of-lambda-kind)
+   (kind (implies (equal kind 'ifp)
+                  (and (consp (typed-term->term tterm))
+                       (equal (car (typed-term->term tterm)) 'if)))
+         :name implies-of-if-kind)
+   (kind (implies (equal kind 'fncallp)
+                  (and (consp (typed-term->term tterm))
+                       (not (equal (car (typed-term->term tterm)) 'quote))
+                       (symbolp (car (typed-term->term tterm)))))
+         :name implies-of-fncall-kind)
+   (kind (implies (equal kind x)
+                  (equal (typed-term->kind
+                          (typed-term (typed-term->term tterm) a b))
+                         x))
+         :name kind-preserved)
+   (kind (implies (not (equal kind x))
+                  (not (equal (typed-term->kind
+                               (typed-term (typed-term->term tterm) a b))
+                              x)))
+         :name not-kind-preserved))
+  (defthm good-typed-fncall-of-0-input-fn
+    (implies (and (symbolp fn)
+                  (not (equal fn 'quote))
+                  (not (equal fn 'if))
+                  (pseudo-termp path-cond)
+                  (pseudo-termp judges))
+             (equal (typed-term->kind
+                     (typed-term `(,fn) path-cond `(if ,judges 't 'nil)))
+                    'fncallp))))
+
+(define good-typed-variable-p ((tterm typed-term-p)
+                               (options type-options-p))
+  :returns (ok booleanp)
+  (b* ((tterm (typed-term-fix tterm))
+       (options (type-options-fix options))
+       ((typed-term tt) tterm)
+       ((type-options to) options))
+    ;; (if (is-conjunct-list? tt.judgements tt.term to.supertype) t nil)
+    t))
+
+#|
+(good-typed-variable-p (typed-term 'x
+''t
+'(if (if (booleanp (rational-integer-alistp x))
+'t
+'nil)
+(if (if 't 't 'nil) 't 'nil)
+'nil)))
+|#
+
+(define good-typed-quote-p ((tterm typed-term-p)
+                            (options type-options-p))
+  :returns (ok booleanp)
+  (b* ((tterm (typed-term-fix tterm))
+       (options (type-options-fix options))
+       ((typed-term tt) tterm)
+       ((type-options to) options))
+    ;; (if (is-conjunct-list? tt.judgements tt.term to.supertype) t nil)
+    t))
+
+#|
+(good-typed-quote-p (typed-term ''t
+''t
+'(if (if (symbolp 't)
+(if (booleanp 't) 't 'nil)
+'nil)
+'t
+'nil)))
+|#
+
+
+;; mrg: I added the test
+;;   (make-typed-term-list-guard actuals tt.path-cond actuals-judge)
+;; to good-typed-lambda-p and good-typed-fncall-p.
+;; This probably creates a verification obligation for the code that
+;; creates judgements for lambdas and function calls.
+(defines good-typed-term
+  :well-founded-relation l<
+  :flag-local nil
+  :verify-guards nil
+  :hints (("Goal"
+           :in-theory (e/d ()
+                           (pseudo-termp
+                            pseudo-term-listp
+                            equal-fixed-and-x-of-pseudo-termp
+                            symbol-listp
+                            acl2::pseudo-termp-cadr-from-pseudo-term-listp))))
+
+  (define good-typed-lambda-p ((tterm typed-term-p)
+                               (options type-options-p))
+    :returns (ok booleanp)
+    :guard (and (consp (typed-term->term tterm))
+                (pseudo-lambdap (car (typed-term->term tterm))))
+    :measure (list (acl2-count (typed-term->term (typed-term-fix tterm)))
+                   0)
+    :ignore-ok t
+    (b* ((tterm (typed-term-fix tterm))
+         (options (type-options-fix options))
+         ((typed-term tt) tterm)
+         ((type-options to) options)
+         ((unless (mbt (and (consp tt.term)
+                            (pseudo-lambdap (car tt.term)))))
+          nil)
+         ((cons fn actuals) tt.term)
+         (formals (lambda-formals fn))
+         (body (lambda-body fn))
+         ((unless (consp tt.judgements)) nil)
+         (match?
+          (case-match tt.judgements
+            (('if return-judge
+                 ('if (('lambda !formals body-judge) . !actuals)
+                     actuals-judge
+                   ''nil)
+               ''nil)
+             (and ;; (is-conjunct-list? return-judge tt.term to.supertype)
+              (make-typed-term-list-guard actuals tt.path-cond actuals-judge) ;; added by mrg
+              (good-typed-term-list-p
+               (make-typed-term-list actuals tt.path-cond actuals-judge)
+               to)
+              (b* ((shadowed-path-cond
+                    (shadow-path-cond formals tt.path-cond))
+                   (substed-actuals-judgements
+                    (term-substitution actuals-judge
+                                       (pairlis$ actuals formals)
+                                       t)))
+                (good-typed-term-p
+                 (make-typed-term :term body
+                                  :path-cond `(if ,shadowed-path-cond
+                                                  ,substed-actuals-judgements
+                                                'nil)
+                                  :judgements body-judge)
+                 to))))
+            (& nil))))
+      (if match? t nil)))
+
+  (define good-typed-if-p ((tterm typed-term-p)
+                           (options type-options-p))
+    :returns (ok booleanp)
+    :guard (and (consp (typed-term->term tterm))
+                (equal (car (typed-term->term tterm)) 'if))
+    :measure (list (acl2-count (typed-term->term (typed-term-fix tterm)))
+                   0)
+    :ignore-ok t
+    (b* ((tterm (typed-term-fix tterm))
+         (options (type-options-fix options))
+         ((typed-term tt) tterm)
+         ((type-options to) options)
+         ((unless (mbt (and (consp tt.term)
+                            (equal (car tt.term) 'if))))
+          nil)
+         ((unless (equal (len (cdr tt.term)) 3))
+          (er hard? 'typed-term=>good-typed-if-p
+              "Malformed if term: ~q0" tt.term))
+         ((list & cond then else) tt.term)
+         ((unless (consp tt.judgements)) nil)
+         (match?
+          (case-match tt.judgements
+            (('if judge-if-top
+                 ('if judge-cond
+                     ('if !cond judge-then judge-else)
+                   ''nil)
+               ''nil)
+             (and ;; (is-conjunct-list? judge-if-top tt.term to.supertype)
+              (good-typed-term-p
+               (make-typed-term :term cond
+                                :path-cond tt.path-cond
+                                :judgements judge-cond)
+               to)
+              (good-typed-term-p
+               (make-typed-term :term then
+                                :path-cond
+                                `(if ,(simple-transformer cond)
+                                     ,tt.path-cond 'nil)
+                                :judgements judge-then)
+               to)
+              (good-typed-term-p
+               (make-typed-term :term else
+                                :path-cond
+                                `(if ,(simple-transformer `(not ,cond))
+                                     ,tt.path-cond 'nil)
+                                :judgements judge-else)
+               to)))
+            (& nil))))
+      (if match? t nil)))
+
+  (define good-typed-fncall-p ((tterm typed-term-p)
+                               (options type-options-p))
+    :returns (ok booleanp)
+    :guard (and (consp (typed-term->term tterm))
+                (not (equal (car (typed-term->term tterm)) 'quote))
+                (symbolp (car (typed-term->term tterm))))
+    :measure (list (acl2-count (typed-term->term (typed-term-fix tterm)))
+                   0)
+    :ignore-ok t
+    (b* ((tterm (typed-term-fix tterm))
+         (options (type-options-fix options))
+         ((typed-term tt) tterm)
+         ((type-options to) options)
+         ((unless (mbt (consp tt.term))) nil)
+         ((cons & actuals) tt.term)
+         ((unless (consp tt.judgements)) nil)
+         (match?
+          (case-match tt.judgements
+            (('if return-judge actuals-judge ''nil)
+             (and ;; (is-conjunct-list? return-judge tt.term to.supertype)
+              (make-typed-term-list-guard actuals tt.path-cond actuals-judge) ;; added by mrg
+              (good-typed-term-list-p
+               (make-typed-term-list actuals tt.path-cond actuals-judge)
+               options)))
+            (& nil))))
+      (if match? t nil)))
+
+  (define good-typed-term-p ((tterm typed-term-p)
+                             (options type-options-p))
+    :returns (ok booleanp)
+    :measure (list (acl2-count (typed-term->term (typed-term-fix tterm)))
+                   1)
+    (b* ((tterm (typed-term-fix tterm))
+         ((typed-term tt) tterm)
+         ((if (equal (typed-term->kind tt) 'variablep))
+          (good-typed-variable-p tt options))
+         ((if (equal (typed-term->kind tt) 'quotep))
+          (good-typed-quote-p tt options))
+         ((if (equal (typed-term->kind tt) 'lambdap))
+          (good-typed-lambda-p tt options))
+         ((if (equal (typed-term->kind tt) 'ifp))
+          (good-typed-if-p tt options)))
+      (good-typed-fncall-p tt options)))
+
+  (define good-typed-term-list-p ((tterm-lst typed-term-list-p)
+                                  (options type-options-p))
+    :returns (ok booleanp)
+    :measure (list (acl2-count
+                    (typed-term-list->term-lst
+                     (typed-term-list-fix tterm-lst)))
+                   1)
+    :hints (("Goal"
+             :in-theory (enable typed-term-list->term-lst)))
+    (b* ((tterm-lst (typed-term-list-fix tterm-lst))
+         ((unless (consp tterm-lst)) t)
+         ((cons tterm-hd tterm-tl) tterm-lst))
+      (and (good-typed-term-p tterm-hd options)
+           (good-typed-term-list-p tterm-tl options)
+           (if tterm-tl ;; added by mrg -- ensures good-typed-term-list-p => uniform-path-cond?
+               (equal (typed-term->path-cond tterm-hd)
+                      (typed-term-list->path-cond tterm-tl))
+             t))))
+  ///
+  (defthm good-typed-variable-p-of-good-term
+    (implies (and (typed-term-p tterm)
+                  (equal (typed-term->kind tterm) 'variablep))
+             (iff (good-typed-term-p tterm options)
+                  (good-typed-variable-p tterm options))))
+  (defthm good-typed-quote-p-of-good-term
+    (implies (and (typed-term-p tterm)
+                  (equal (typed-term->kind tterm) 'quotep))
+             (iff (good-typed-term-p tterm options)
+                  (good-typed-quote-p tterm options))))
+  (defthm good-typed-lambda-p-of-good-term
+    (implies (and (typed-term-p tterm)
+                  (equal (typed-term->kind tterm) 'lambdap))
+             (iff (good-typed-term-p tterm options)
+                  (good-typed-lambda-p tterm options))))
+  (defthm good-typed-if-p-of-good-term
+    (implies (and (typed-term-p tterm)
+                  (equal (typed-term->kind tterm) 'ifp))
+             (iff (good-typed-term-p tterm options)
+                  (good-typed-if-p tterm options))))
+  (defthm good-typed-fncall-p-of-good-term
+    (implies (and (typed-term-p tterm)
+                  (equal (typed-term->kind tterm) 'fncallp))
+             (iff (good-typed-term-p tterm options)
+                  (good-typed-fncall-p tterm options))))
+  (defthm good-typed-term-list-of-nil
+    (good-typed-term-list-p nil options))
+  )
+
+(local (in-theory (disable pseudo-termp
+                           symbol-listp
+                           acl2::pseudo-termp-opener
+                           pseudo-term-listp-of-symbol-listp)))
+
+(verify-guards good-typed-term-p)
+
+;; mrg: I added uniform-path-help-when-good-typed-term-list-p and
+;;   uniform-path-cond?-when-good-typed-term-list-p.  These are really
+;;   more-returns theorems of good-typed-term-listp, but when I try to
+;;   state them as such, the proofs take much longer and then fail.
+;;   I'm guessing that ACL2 gets lost when pseudo-termp is enabled.
+;;   Rather figuring out the various theory hints that would make it
+;;   work, I'm just stating the theorems here.
+;;     Note that uniform-path-help-when-good-typed-term-list-p conjures up
+;;   path-cond as a free variable that just happens to be equal to
+;;     (typed-term-list->path-cond tterm-lst).  I suspect this will make it
+;;   hard to apply the rule automatically, but it still may be useful in
+;;   subsequent arguments about good-typed-term-list-p and
+;;   uniform-path-cond?.  Thus, I'm admitting it as a disabled theorem.
+(defthmd uniform-path-help-when-good-typed-term-list-p
+  (implies (and (typed-term-list-p tterm-lst)
+                (good-typed-term-list-p tterm-lst options)
+                (equal (typed-term-list->path-cond tterm-lst) path-cond))
+           (uniform-path-help tterm-lst path-cond))
+  :hints(("Goal"
+          :in-theory (enable good-typed-term-list-p uniform-path-help typed-term-list->path-cond))))
+
+(defthm uniform-path-cond?-when-good-typed-term-list-p
+  (implies (and (typed-term-list-p tterm-lst)
+                (good-typed-term-list-p tterm-lst options))
+           (uniform-path-cond? tterm-lst))
+  :hints(("Goal"
+          :in-theory (enable uniform-path-cond?)
+          :use((:instance uniform-path-help-when-good-typed-term-list-p
+                          (path-cond (typed-term-list->path-cond tterm-lst)))))))
+
+;; mrg:  I added the hypothesis
+;;         (equal (typed-term->path-cond tterm)
+;;                (typed-term-list->path-cond tterm-lst))
+;;  which is required to ensure uniform-path-cond?
+(defthm good-typed-term-list-of-cons
+  (implies (and (type-options-p options)
+                (typed-term-p tterm)
+                (good-typed-term-p tterm options)
+                (typed-term-list-p tterm-lst)
+                (good-typed-term-list-p tterm-lst options)
+                (equal (typed-term->path-cond tterm)
+                       (typed-term-list->path-cond tterm-lst)))
+           (good-typed-term-list-p (cons tterm tterm-lst) options))
+  :hints (("Goal"
+           :in-theory (enable good-typed-term-list-p)
+           :expand (good-typed-term-list-p (cons tterm tterm-lst) options))))
+
+(defthm good-typed-term-of-car
+  (implies (and (type-options-p options)
+                (typed-term-list-p tterm-lst)
+                (good-typed-term-list-p tterm-lst options)
+                (consp tterm-lst))
+           (good-typed-term-p (car tterm-lst) options))
+  :hints (("Goal"
+           :in-theory (enable good-typed-term-list-p)
+           :expand (good-typed-term-list-p tterm-lst options))))
+
+(defthm good-typed-term-list-of-cdr
+  (implies (and (type-options-p options)
+                (typed-term-list-p tterm-lst)
+                (good-typed-term-list-p tterm-lst options)
+                (consp tterm-lst))
+           (good-typed-term-list-p (cdr tterm-lst) options))
+  :hints (("Goal"
+           :in-theory (enable good-typed-term-list-p)
+           :expand (good-typed-term-list-p tterm-lst options))))
+
+
+(defthm good-typed-term-list-of-make-typed-term-list
+  (implies (and (typed-term-list-p tterm-lst)
+                (type-options-p options)
+                (good-typed-term-list-p tterm-lst options))
+           (good-typed-term-list-p
+            (make-typed-term-list (typed-term-list->term-lst tterm-lst)
+                                  (typed-term-list->path-cond tterm-lst)
+                                  (typed-term-list->judgements tterm-lst))
+            options)))
+
+(defthm good-typed-term-of-make-typed-term
+  (good-typed-term-p (make-typed-term) options)
+  :hints (("Goal" :in-theory (enable good-typed-term-p
+                                     good-typed-quote-p
+                                     is-conjunct-list?
+                                     judgement-of-term))))
+
+(defthm good-typed-term-of-make-typed-term-list-with-path-cond
+  (good-typed-term-list-p (make-typed-term-list nil path-cond ''t)
+                          options)
+  :hints (("Goal" :in-theory (enable good-typed-term-list-p
+                                     make-typed-term-list))))
+
+(local
+ (defthm crock
+   (implies (pseudo-termp judges)
+            (and (pseudo-termp `(if ,judges 't 'nil))
+                 (consp `(if ,judges 't 'nil))
+                 (consp (cdddr `(if ,judges 't 'nil))))))
+ )
+
+(defthm good-typed-term-of-0-input-fn
+  (implies (and (symbolp fn)
+                (not (equal fn 'quote))
+                (not (equal fn 'if))
+                (pseudo-termp path-cond)
+                (pseudo-termp judges)
+                (type-options-p options))
+           (good-typed-term-p
+            (typed-term `(,fn) path-cond `(if ,judges 't 'nil))
+            options))
+  :hints (("Goal"
+           :in-theory (enable pseudo-termp good-typed-term-list-p)
+           :expand (good-typed-fncall-p
+                    (typed-term `(,fn) path-cond `(if ,judges 't 'nil))
+                    options))))
+
+;; -------------------------------------------------------------------
+;; Theorems for destructors
+;; TODO: simplify the proof
+
+(defthm implies-of-good-typed-if
+  (implies (and (typed-term-p tterm) (type-options-p options)
+                (good-typed-if-p tterm options))
+           (and (consp (cdr (typed-term->term tterm)))
+                (consp (cddr (typed-term->term tterm)))
+                (consp (cdddr (typed-term->term tterm)))
+                (consp (typed-term->judgements tterm))
+                (consp (cdr (typed-term->judgements tterm)))
+                (consp (cddr (typed-term->judgements tterm)))
+                (consp (caddr (typed-term->judgements tterm)))
+                (consp (cdddr (typed-term->judgements tterm)))
+                (not (cddddr (typed-term->judgements tterm)))
+                (consp (cdr (caddr (typed-term->judgements tterm))))
+                (consp (cddr (caddr (typed-term->judgements tterm))))
+                (consp (caddr (caddr (typed-term->judgements tterm))))
+                (consp (cddr (caddr (caddr (typed-term->judgements tterm)))))
+                (consp (cdr (caddr (caddr (typed-term->judgements tterm)))))
+                (consp (cdddr (caddr (typed-term->judgements tterm))))
+                (not (cddddr (caddr (typed-term->judgements tterm))))
+                (consp (cdddr (caddr (caddr (typed-term->judgements tterm)))))
+                (not (cddddr (caddr (caddr (typed-term->judgements tterm)))))
+                (pseudo-termp (cadr (typed-term->judgements tterm)))
+                (pseudo-termp (cadr (caddr (typed-term->judgements tterm))))
+                (good-typed-term-p
+                 (typed-term (cadr (typed-term->term tterm))
+                             (typed-term->path-cond tterm)
+                             (cadr (caddr (typed-term->judgements tterm))))
+                 options)
+                (good-typed-term-p
+                 (typed-term (caddr (typed-term->term tterm))
+                             (list* 'if
+                                    (simple-transformer (cadr (typed-term->term tterm)))
+                                    (typed-term->path-cond tterm)
+                                    '('nil))
+                             (caddr (caddr (caddr (typed-term->judgements
+                                                   tterm)))))
+                 options)
+                (good-typed-term-p
+                 (typed-term
+                  (cadddr (typed-term->term tterm))
+                  (list* 'if
+                         (simple-transformer (list 'not
+                                                   (cadr (typed-term->term tterm))))
+                         (typed-term->path-cond tterm)
+                         '('nil))
+                  (cadddr (caddr (caddr (typed-term->judgements tterm)))))
+                 options)
+                (pseudo-termp (caddr (caddr (caddr (typed-term->judgements
+                                                    tterm)))))
+                (pseudo-termp (cadddr (caddr (caddr (typed-term->judgements
+                                                     tterm)))))))
+  :hints (("Goal"
+           :expand (good-typed-if-p tterm options))))
+
+(defthm implies-of-good-typed-fncall
+  (implies (and (typed-term-p tterm) (type-options-p options)
+                (good-typed-fncall-p tterm options))
+           (and (consp (typed-term->judgements tterm))
+                (consp (cdr (typed-term->judgements tterm)))
+                (consp (cddr (typed-term->judgements tterm)))
+                (consp (cdddr (typed-term->judgements tterm)))
+                (pseudo-termp (cadr (typed-term->judgements tterm)))
+                (pseudo-termp (caddr (typed-term->judgements tterm)))
+                (not (cddddr (typed-term->judgements tterm)))
+                (good-typed-term-list-p
+                 (make-typed-term-list (cdr (typed-term->term tterm))
+                                       (typed-term->path-cond tterm)
+                                       (caddr (typed-term->judgements tterm)))
+                 options)))
+  :hints (("Goal"
+           :expand (good-typed-fncall-p tterm options))))
+
+(defthm implies-of-good-typed-lambda
+  (implies (and (typed-term-p tterm) (type-options-p options)
+                (good-typed-lambda-p tterm options))
+           (and (consp (typed-term->judgements tterm))
+                (consp (cdr (typed-term->judgements tterm)))
+                (consp (caddr (typed-term->judgements tterm)))
+                (consp (cddr (typed-term->judgements tterm)))
+                (consp (cdddr (typed-term->judgements tterm)))
+                (consp (cadr (caddr (typed-term->judgements tterm))))
+                (consp (car (cadr (caddr (typed-term->judgements tterm)))))
+                (consp (cdr (caddr (typed-term->judgements tterm))))
+                (consp (cdr (car (cadr (caddr (typed-term->judgements tterm))))))
+                (consp (cddr (caddr (typed-term->judgements tterm))))
+                (consp (cdddr (caddr (typed-term->judgements tterm))))
+                (consp (cddr (car (cadr (caddr (typed-term->judgements tterm))))))
+                (not (cddddr (typed-term->judgements tterm)))
+                (not (cddddr (caddr (typed-term->judgements tterm))))
+                (not (cdddr (car (cadr (caddr (typed-term->judgements
+                                               tterm))))))
+                (pseudo-termp (cadr (typed-term->judgements tterm)))
+                (good-typed-term-list-p
+                 (make-typed-term-list (cdr (typed-term->term tterm))
+                                       (typed-term->path-cond tterm)
+                                       (caddr (caddr (typed-term->judgements
+                                                      tterm))))
+                 options)
+                (good-typed-term-p
+                 (typed-term (caddr (car (typed-term->term tterm)))
+                             (list* 'if
+                                    (shadow-path-cond (cadr (car (typed-term->term tterm)))
+                                                      (typed-term->path-cond tterm))
+                                    (term-substitution (caddr (caddr (typed-term->judgements tterm)))
+                                                       (pairlis$ (cdr (typed-term->term tterm))
+                                                                 (cadr (car (typed-term->term tterm))))
+                                                       t)
+                                    '('nil))
+                             (caddr (car (cadr (caddr (typed-term->judgements tterm))))))
+                 options)))
+  :hints (("Goal"
+           :expand (good-typed-lambda-p tterm options))))
+
+;; ---------------------------------------------
+;;       Destructors for typed-terms
+(local (in-theory (disable (:executable-counterpart typed-term))))
+
+;; ifp destructors
+(define typed-term-if->cond ((tterm typed-term-p)
+                             (options type-options-p))
+  :guard (and (equal (typed-term->kind tterm) 'ifp)
+              (good-typed-term-p tterm options))
+  :returns (new-tt (and (typed-term-p new-tt)
+                        (good-typed-term-p new-tt options)))
+  (b* (((unless (mbt (and (typed-term-p tterm)
+                          (type-options-p options)
+                          (equal (typed-term->kind tterm) 'ifp)
+                          (good-typed-term-p tterm options))))
+        (make-typed-term))
+       ((typed-term tt) tterm)
+       (cond-term (cadr tt.term))
+       (cond-path-cond tt.path-cond)
+       ((mv err cond-judgements)
+        (case-match tt.judgements
+          ((& & (& judge-cond . &) &)
+           (mv nil judge-cond))
+          (& (mv t nil))))
+       ((if err)
+        (er hard? 'typed-term=>typed-term-if->cond
+            "Malformed if judgements ~q0" tt.judgements)))
+    (make-typed-term :term cond-term
+                     :path-cond cond-path-cond
+                     :judgements cond-judgements))
+  ///
+  (more-returns
+   (new-tt (implies
+            (and (typed-term-p tterm)
+                 (type-options-p options)
+                 (equal (typed-term->kind tterm) 'ifp)
+                 (good-typed-term-p tterm options))
+            (< (acl2-count (typed-term->term new-tt))
+               (acl2-count (typed-term->term tterm))))
+           :name acl2-count-of-typed-term-if->cond)))
+
+(define typed-term-if->then ((tterm typed-term-p)
+                             (options type-options-p))
+  :guard (and (equal (typed-term->kind tterm) 'ifp)
+              (good-typed-term-p tterm options))
+  :returns (new-tt (and (typed-term-p new-tt)
+                        (good-typed-term-p new-tt options)))
+  (b* (((unless (mbt (and (typed-term-p tterm)
+                          (type-options-p options)
+                          (equal (typed-term->kind tterm) 'ifp)
+                          (good-typed-term-p tterm options))))
+        (make-typed-term))
+       ((typed-term tt) tterm)
+       ((list* & cond then-term &) tt.term)
+       (then-path-cond `(if ,(simple-transformer cond)
+                            ,tt.path-cond 'nil))
+       ((mv err then-judgements)
+        (case-match tt.judgements
+          ((& & (& & (& & judge-then . &) &) &)
+           (mv nil judge-then))
+          (& (mv t nil))))
+       ((if err)
+        (er hard? 'typed-term=>typed-term-if->then
+            "Malformed if judgements ~q0" tt.judgements)))
+    (make-typed-term :term then-term
+                     :path-cond then-path-cond
+                     :judgements then-judgements))
+  ///
+  (more-returns
+   (new-tt (implies
+            (and (typed-term-p tterm)
+                 (type-options-p options)
+                 (equal (typed-term->kind tterm) 'ifp)
+                 (good-typed-term-p tterm options))
+            (< (acl2-count (typed-term->term new-tt))
+               (acl2-count (typed-term->term tterm))))
+           :name acl2-count-of-typed-term-if->then)))
+
+(define typed-term-if->else ((tterm typed-term-p)
+                             (options type-options-p))
+  :guard (and (equal (typed-term->kind tterm) 'ifp)
+              (good-typed-term-p tterm options))
+  :returns (new-tt (and (typed-term-p new-tt) (good-typed-term-p new-tt options)))
+  (b* (((unless (mbt (and (typed-term-p tterm)
+                          (type-options-p options)
+                          (equal (typed-term->kind tterm) 'ifp)
+                          (good-typed-term-p tterm options))))
+        (make-typed-term))
+       ((typed-term tt) tterm)
+       ((list & cond & else-term) tt.term)
+       (else-path-cond `(if ,(simple-transformer `(not ,cond))
+                            ,tt.path-cond 'nil))
+       ((mv err else-judgements)
+        (case-match tt.judgements
+          ((& & (& & (& & & judge-else) &) &)
+           (mv nil judge-else))
+          (& (mv t nil))))
+       ((if err)
+        (er hard? 'typed-term=>typed-term-if->else
+            "Malformed if judgements ~q0" tt.judgements)))
+    (make-typed-term :term else-term
+                     :path-cond else-path-cond
+                     :judgements else-judgements))
+  ///
+  (more-returns
+   (new-tt (implies
+            (and (typed-term-p tterm)
+                 (type-options-p options)
+                 (equal (typed-term->kind tterm) 'ifp)
+                 (good-typed-term-p tterm options))
+            (< (acl2-count (typed-term->term new-tt))
+               (acl2-count (typed-term->term tterm))))
+           :name acl2-count-of-typed-term-if->else)))
+
+(define typed-term->top ((tterm typed-term-p)
+                         (options type-options-p))
+  :guard (and (or (equal (typed-term->kind tterm) 'ifp)
+                  (equal (typed-term->kind tterm) 'lambdap)
+                  (equal (typed-term->kind tterm) 'fncallp))
+              (good-typed-term-p tterm options))
+  :returns (new-tt typed-term-p)
+  (b* (((unless (mbt (and (typed-term-p tterm)
+                          (type-options-p options)
+                          (or (equal (typed-term->kind tterm) 'ifp)
+                              (equal (typed-term->kind tterm) 'lambdap)
+                              (equal (typed-term->kind tterm) 'fncallp))
+                          (good-typed-term-p tterm options))))
+        (make-typed-term))
+       ((typed-term tt) tterm)
+       ((mv err top-judge)
+        (case-match tt.judgements
+          ((& top-judge & &)
+           (mv nil top-judge))
+          (& (mv t nil))))
+       ((if err)
+        (prog2$ (er hard? 'typed-term=>typed-term->top
+                    "Malformed judgements ~q0" tt.judgements)
+                (make-typed-term))))
+    (make-typed-term :term tt.term
+                     :path-cond tt.path-cond
+                     :judgements top-judge))
+  ///
+  (more-returns
+   (new-tt (implies (and (equal (typed-term->kind tterm)
+                                'lambdap)
+                         (good-typed-term-p tterm options)
+                         (typed-term-p tterm)
+                         (type-options-p options))
+                    (and (consp (typed-term->term new-tt))
+                         (pseudo-lambdap (car (typed-term->term new-tt)))))
+           :name implies-of-typed-term->top)))
+
+;; fncallp destructors
+(define typed-term-fncall->actuals ((tterm typed-term-p)
+                                    (options type-options-p))
+  :guard (and (equal (typed-term->kind tterm) 'fncallp)
+              (good-typed-term-p tterm options))
+  :guard-hints (("Goal"
+                 :expand (good-typed-fncall-p tterm options)))
+  :returns (new-ttl (and (typed-term-list-p new-ttl)
+                         (good-typed-term-list-p new-ttl options)))
+  (b* (((unless (mbt (and (typed-term-p tterm)
+                          (type-options-p options)
+                          (equal (typed-term->kind tterm) 'fncallp)
+                          (good-typed-term-p tterm options))))
+        nil)
+       ((typed-term tt) tterm)
+       ((cons & actuals) tt.term)
+       ((mv err actuals-judgements)
+        (case-match tt.judgements
+          ((& & actuals-judge . &)
+           (mv nil actuals-judge))
+          (& (mv t nil))))
+       ((if err)
+        (er hard? 'typed-term=>typed-term-fncall->actuals
+            "Malformed fncall judgements ~q0" tt.judgements)))
+    (make-typed-term-list actuals tt.path-cond actuals-judgements))
+  ///
+  (more-returns
+   (new-ttl (implies (and (typed-term-p tterm)
+                          (type-options-p options)
+                          (equal (typed-term->kind tterm) 'fncallp)
+                          (good-typed-term-p tterm options))
+                     (< (acl2-count
+                         (typed-term-list->term-lst new-ttl))
+                        (acl2-count (typed-term->term tterm))))
+            :name acl2-count-of-make-typed-fncall)))
+
+;; lambdap destructors
+(define typed-term-lambda->actuals ((tterm typed-term-p)
+                                    (options type-options-p))
+  :guard (and (equal (typed-term->kind tterm) 'lambdap)
+              (good-typed-term-p tterm options))
+  :guard-hints (("Goal"
+                 :expand (good-typed-lambda-p tterm options)))
+  :returns (new-ttl (and (typed-term-list-p new-ttl)
+                         (good-typed-term-list-p new-ttl options)))
+  (b* (((unless (mbt (and (typed-term-p tterm)
+                          (type-options-p options)
+                          (equal (typed-term->kind tterm) 'lambdap)
+                          (good-typed-term-p tterm options))))
+        nil)
+       ((typed-term tt) tterm)
+       ((cons & actuals) tt.term)
+       ((mv err actuals-judgements)
+        (case-match tt.judgements
+          ((& & (& & actuals-judge . &) &)
+           (mv nil actuals-judge))
+          (& (mv t nil))))
+       ((if err)
+        (er hard? 'typed-term=>typed-term-lambda->actuals
+            "Malformed lambda judgements ~q0" tt.judgements)))
+    (make-typed-term-list actuals tt.path-cond actuals-judgements))
+  ///
+  (more-returns
+   (new-ttl (implies (and (typed-term-p tterm)
+                          (equal (typed-term->kind tterm)
+                                 'lambdap)
+                          (good-typed-term-p tterm options))
+                     (< (acl2-count
+                         (typed-term-list->term-lst new-ttl))
+                        (acl2-count (typed-term->term tterm))))
+            :name acl2-count-of-typed-term-lambda->actuals)
+   ;; (new-ttl (implies (and (typed-term-p tterm)
+   ;;                        (type-options-p options)
+   ;;                        (equal (typed-term->kind tterm)
+   ;;                               'lambdap)
+   ;;                        (good-typed-term-p tterm options))
+   ;;                   (equal (len (cdr (typed-term->term tterm)))
+   ;;                          (len (typed-term-list->term-lst new-ttl))))
+   ;;          :name typed-term-lambda->actuals-preserve-len
+   ;;          :hints (("Goal"
+   ;;                   :in-theory (enable typed-term-list->term-lst)
+   ;;                   :expand (typed-term-lambda->actuals tterm options))))
+   ))
+
+(define typed-term-lambda->body ((tterm typed-term-p)
+                                 (options type-options-p))
+  :guard (and (equal (typed-term->kind tterm) 'lambdap)
+              (good-typed-term-p tterm options))
+  :guard-hints (("Goal"
+                 :expand (good-typed-lambda-p tterm options)))
+  :returns (new-tt (and (typed-term-p new-tt)
+                        (good-typed-term-p new-tt options)))
+  (b* (((unless (mbt (and (typed-term-p tterm)
+                          (type-options-p options)
+                          (equal (typed-term->kind tterm) 'lambdap)
+                          (good-typed-term-p tterm options))))
+        (make-typed-term))
+       ((typed-term tt) tterm)
+       ((cons fn actuals) tt.term)
+       (formals (lambda-formals fn))
+       (body (lambda-body fn))
+       (shadowed-path-cond (shadow-path-cond formals tt.path-cond))
+       ((mv err body-judgements actuals-judges)
+        (case-match tt.judgements
+          ((& & (& ((& & body-judge) . &) actuals-judges &) &)
+           (mv nil body-judge actuals-judges))
+          (& (mv t nil nil))))
+       ((if err)
+        (er hard? 'typed-term=>typed-term-lambda->body
+            "Malformed lambda judgements ~q0" tt.judgements))
+       (substed-actuals-judgements
+        (term-substitution actuals-judges (pairlis$ actuals formals) t)))
+    (make-typed-term :term body
+                     :path-cond `(if ,shadowed-path-cond
+                                     ,substed-actuals-judgements 'nil)
+                     :judgements body-judgements))
+  ///
+  (more-returns
+   (new-tt (implies (and (typed-term-p tterm)
+                         (type-options-p options)
+                         (equal (typed-term->kind tterm)
+                                'lambdap)
+                         (good-typed-term-p tterm options))
+                    (< (acl2-count (typed-term->term new-tt))
+                       (acl2-count (typed-term->term tterm))))
+           :name acl2-count-of-typed-term-lambda->body)))
+
+;; --------------------------------------------------------------------
+;;      Constructors
+
+(defthm kind-of-make-typed-if
+  (implies
+   (and (typed-term-p tt-top)
+        (typed-term-p tt-cond)
+        (typed-term-p tt-then)
+        (typed-term-p tt-else)
+        (good-typed-term-p tt-cond options)
+        (good-typed-term-p tt-then options)
+        (good-typed-term-p tt-else options))
+   (equal (typed-term->kind
+           (typed-term (list 'if
+                             (typed-term->term tt-cond)
+                             (typed-term->term tt-then)
+                             (typed-term->term tt-else))
+                       (typed-term->path-cond tt-top)
+                       (list* 'if
+                              (typed-term->judgements tt-top)
+                              (list* 'if
+                                     (typed-term->judgements tt-cond)
+                                     (list 'if
+                                           (typed-term->term tt-cond)
+                                           (typed-term->judgements tt-then)
+                                           (typed-term->judgements tt-else))
+                                     '('nil))
+                              '('nil))))
+          'ifp))
+  :hints (("Goal"
+           :in-theory (enable typed-term->kind))))
+
+(define make-typed-if ((tt-top typed-term-p)
+                       (tt-cond typed-term-p)
+                       (tt-then typed-term-p)
+                       (tt-else typed-term-p)
+                       (options type-options-p))
+  :guard (and (good-typed-term-p tt-cond options)
+              (good-typed-term-p tt-then options)
+              (good-typed-term-p tt-else options))
+  :returns (new-tt (and (typed-term-p new-tt)
+                        (good-typed-term-p new-tt options))
+                   :hints (("Goal"
+                            :in-theory (enable good-typed-if-p))))
+  (b* (((unless (mbt (and (type-options-p options)
+                          (typed-term-p tt-top)
+                          (typed-term-p tt-cond)
+                          (typed-term-p tt-then)
+                          (typed-term-p tt-else)
+                          (good-typed-term-p tt-cond options)
+                          (good-typed-term-p tt-then options)
+                          (good-typed-term-p tt-else options))))
+        (make-typed-term))
+       ((typed-term ttp) tt-top)
+       ((typed-term ttc) tt-cond)
+       ((typed-term ttt) tt-then)
+       ((typed-term tte) tt-else)
+       ((unless (and (equal ttc.path-cond ttp.path-cond)
+                     (equal ttt.path-cond
+                            `(if ,(simple-transformer ttc.term)
+                                 ,ttc.path-cond 'nil))
+                     (equal tte.path-cond
+                            `(if ,(simple-transformer `(not ,ttc.term))
+                                 ,ttc.path-cond 'nil))))
+        (prog2$
+         (er hard? 'typed-term=>make-typed-term-if
+             "Inconsistent inputs.~%")
+         (make-typed-term))))
+    (make-typed-term
+     :term `(if ,ttc.term ,ttt.term ,tte.term)
+     :path-cond ttp.path-cond
+     :judgements
+     `(if ,ttp.judgements
+          (if ,ttc.judgements
+              (if ,ttc.term ,ttt.judgements ,tte.judgements)
+            'nil)
+        'nil))))
+
+(local
+ (defthm pseudo-termp-of-lambda
+   (implies (and (symbol-listp formals)
+                 (pseudo-termp body-judge)
+                 (pseudo-term-listp actuals)
+                 (equal (len formals) (len actuals)))
+            (pseudo-termp
+             `((lambda ,formals ,body-judge) ,@actuals)))
+   :hints (("Goal"
+            :in-theory (enable pseudo-termp))))
+ )
+
+(defthm kind-of-make-typed-lambda
+  (implies
+   (and (typed-term-p tt-top)
+        (typed-term-p tt-body)
+        (typed-term-list-p tt-actuals)
+        (good-typed-term-p tt-body options)
+        (good-typed-term-list-p tt-actuals options)
+        (pseudo-lambdap (car (typed-term->term tt-top))))
+   (equal (typed-term->kind
+           (typed-term
+            (typed-term->term tt-top)
+            (typed-term->path-cond tt-top)
+            (list* 'if
+                   (typed-term->judgements tt-top)
+                   (list* 'if
+                          (cons (list 'lambda
+                                      (cadr (car (typed-term->term tt-top)))
+                                      (typed-term->judgements tt-body))
+                                (typed-term-list->term-lst tt-actuals))
+                          (typed-term-list->judgements tt-actuals)
+                          '('nil))
+                   '('nil))))
+          'lambdap))
+  :hints (("Goal"
+           :in-theory (enable typed-term->kind))))
+
+(define make-typed-lambda ((tt-top typed-term-p)
+                           (tt-body typed-term-p)
+                           (tt-actuals typed-term-list-p)
+                           (options type-options-p))
+  :guard (and (good-typed-term-p tt-body options)
+              (good-typed-term-list-p tt-actuals options))
+  :returns (new-tt (and (typed-term-p new-tt)
+                        (good-typed-term-p new-tt options))
+                   :hints (("Goal"
+                            :in-theory (enable good-typed-lambda-p))))
+  (b* (((unless (mbt (and (type-options-p options)
+                          (typed-term-p tt-top)
+                          (typed-term-p tt-body)
+                          (typed-term-list-p tt-actuals)
+                          (good-typed-term-p tt-body options)
+                          (good-typed-term-list-p tt-actuals options))))
+        (make-typed-term))
+       ((typed-term ttt) tt-top)
+       ((typed-term ttb) tt-body)
+       (tta.term-lst (typed-term-list->term-lst tt-actuals))
+       (tta.path-cond (typed-term-list->path-cond tt-actuals))
+       (tta.judgements (typed-term-list->judgements tt-actuals))
+       ((unless (and (consp ttt.term)
+                     (pseudo-lambdap (car ttt.term))))
+        (prog2$ (er hard? 'typed-term=>make-typed-term-lambda
+                    "Inconsistent inputs.~%")
+                (make-typed-term)))
+       (formals (lambda-formals (car ttt.term)))
+       (body (lambda-body (car ttt.term)))
+       (actuals (cdr ttt.term))
+       (body-path-cond
+        `(if ,(shadow-path-cond formals ttt.path-cond)
+             ,(term-substitution tta.judgements
+                                 (pairlis$ tta.term-lst formals) t)
+           'nil))
+       (- (cw "formals: ~p0 actuals ~p1 body: ~p2~%" formals actuals body))
+       (- (cw "tta.term-lst: ~q0" tta.term-lst))
+       (- (cw "ttb.path-cond: ~q0" ttb.path-cond))
+       (- (cw "ttb.term: ~q0" ttb.term))
+       (- (cw "body-path-cond: ~q0" body-path-cond))
+       (- (cw "ttt.path-cond: ~q0" ttt.path-cond))
+       (- (cw "tta.path-cond: ~q0" tta.path-cond))
+       ((unless (and (equal tta.term-lst actuals)
+                     (equal body ttb.term)
+                     (equal (len formals) (len actuals))
+                     (equal ttb.path-cond body-path-cond)
+                     (equal ttt.path-cond tta.path-cond)))
+        (prog2$ (er hard? 'typed-term=>make-typed-term-lambda
+                    "Inconsistent inputs.~%")
+                (make-typed-term))))
+    (make-typed-term
+     :term ttt.term
+     :path-cond ttt.path-cond
+     :judgements `(if ,ttt.judgements
+                      (if ((lambda ,formals
+                             ,ttb.judgements)
+                           ,@actuals)
+                          ,tta.judgements
+                        'nil)
+                    'nil))))
+
+(defthm kind-of-make-typed-fncall
+  (implies
+   (and (typed-term-p tt-top)
+        (typed-term-list-p tt-actuals)
+        (good-typed-term-list-p tt-actuals options)
+        (consp (typed-term->term tt-top))
+        (symbolp (car (typed-term->term tt-top)))
+        (not (equal (car (typed-term->term tt-top)) 'quote))
+        (not (equal (car (typed-term->term tt-top)) 'if))
+        (equal (cdr (typed-term->term tt-top))
+               (typed-term-list->term-lst tt-actuals))
+        (equal (typed-term->path-cond tt-top)
+               (typed-term-list->path-cond tt-actuals)))
+   (equal (typed-term->kind
+           (typed-term (typed-term->term tt-top)
+                       (typed-term->path-cond tt-top)
+                       (list* 'if
+                              (typed-term->judgements tt-top)
+                              (typed-term-list->judgements tt-actuals)
+                              '('nil))))
+          'fncallp))
+  :hints (("Goal"
+           :in-theory (enable typed-term->kind))))
+
+(define make-typed-fncall ((tt-top typed-term-p)
+                           (tt-actuals typed-term-list-p)
+                           (options type-options-p))
+  :guard (good-typed-term-list-p tt-actuals options)
+  :returns (new-tt (and (typed-term-p new-tt)
+                        (good-typed-term-p new-tt options))
+                   :hints (("Goal"
+                            :in-theory (enable good-typed-fncall-p))))
+  (b* (((unless (mbt (and (typed-term-p tt-top)
+                          (typed-term-list-p tt-actuals)
+                          (type-options-p options)
+                          (good-typed-term-list-p tt-actuals options))))
+        (make-typed-term))
+       ((typed-term ttt) tt-top)
+       (tta.term-lst (typed-term-list->term-lst tt-actuals))
+       (tta.path-cond (typed-term-list->path-cond tt-actuals))
+       (tta.judgements (typed-term-list->judgements tt-actuals))
+       ((unless (and (consp ttt.term)
+                     (symbolp (car ttt.term))
+                     (equal (cdr ttt.term) tta.term-lst)
+                     (equal ttt.path-cond tta.path-cond)
+                     (not (equal (car ttt.term) 'quote))
+                     (not (equal (car ttt.term) 'if))))
+        (prog2$ (er hard? 'typed-term=>make-typed-fncall
+                    "Inconsistent inputs.~%")
+                (make-typed-term))))
+    (make-typed-term
+     :term ttt.term
+     :path-cond ttt.path-cond
+     :judgements `(if ,ttt.judgements ,tta.judgements 'nil))))
